theories/aneris_lang/state_interp/auxiliary_state.v
@@ -1,0 +1,186 @@
+From stdpp Require Import fin_maps gmap option.
+From aneris.prelude Require Import quantifiers.
+From iris.bi.lib Require Import fractional.
+From iris.proofmode Require Import tactics.
+From iris.base_logic.lib Require Import saved_prop gen_heap.
+From iris_string_ident Require Import ltac2_string_ident.
+From aneris.program_logic Require Export weakestpre adequacy.
+From aneris.program_logic Require Import ectx_lifting.
+From aneris.lib Require Import gen_heap_light.
+From aneris.aneris_lang Require Export aneris_lang notation network resources.
+From aneris.aneris_lang.lib Require Import util.
+From aneris.aneris_lang.state_interp Require Import
+     state_interp_def
+     state_interp_network_sockets_coh
+     state_interp_socket_interp_coh
+     state_interp_messages_history_coh.
+
+From RecordUpdate Require Import RecordSet.
+Set Default Proof Using "Type".
+
+Import uPred.
+Import Network.
+Import RecordSetNotations.
+
+Section Aneris_AS.
+  Context `{aG : !anerisG Mdl Σ}.
+
+  Lemma get_buffer_some r sh skt Sn S a :
+    socket_handlers_coh Sn →
+    S !! (ip_of_address a) = Some Sn →
+    Sn !! sh = Some (skt, r) →
+    saddress skt = Some a →
+    get_buffer S a = Some r.
+  Proof.
+    intros Hskcoh HS HSn Hskt. rewrite /get_buffer HS /=.
+    destruct (find _ _) as [[sh' [skt' r']]|] eqn:Hf; simpl in *; last first.
+    { apply elem_of_map_to_list, elem_of_list_In in HSn.
+      eapply find_none in Hf; last done.
+      rewrite bool_decide_eq_true_2 in Hf; done. }
+    apply find_some in Hf as [Hf1 Hf2%bool_decide_eq_true].
+    apply elem_of_list_In, elem_of_map_to_list' in Hf1.
+    simpl in *. assert (sh' = sh) as ->.
+    { apply (Hskcoh sh' sh skt' skt r' r); eauto. rewrite Hskt Hf2; done. }
+    rewrite Hf1 in HSn; simplify_eq; done.
+  Qed.
+
+  Lemma get_buffer_inv r S a :
+    get_buffer S a = Some r →
+    ∃ sh skt Sn,
+    S !! (ip_of_address a) = Some Sn ∧
+    Sn !! sh = Some (skt, r) ∧
+    saddress skt = Some a.
+  Proof.
+    intros Hbuf. rewrite /get_buffer in Hbuf.
+    apply bind_Some in Hbuf as (Sn & HSn & Hfind).
+    apply fmap_Some in Hfind as ((h0,(s0,r0)) & Hfind & ->).
+    apply find_some in Hfind as (Hin & Hbl%bool_decide_eq_true).
+    apply elem_of_list_In, elem_of_map_to_list' in Hin. simpl in *. eauto 9.
+  Qed.
+
+
+  Lemma get_buffer_deliver_message S M Sn sh skt a r m :
+    let S' := (<[ip_of_address a := (<[sh:=(skt, r ∪ {[m]})]> Sn) ]> S) in
+    m ∈ messages_to_receive_at a M →
+    S !! (ip_of_address a) = Some Sn →
+    Sn !! sh = Some (skt, r) →
+    saddress skt = Some a →
+    socket_handlers_coh Sn  →
+    get_buffer S' a = Some (r ∪ {[m]}).
+  Proof.
+    simpl. intros ?????. eapply (get_buffer_some _ sh) ;
+      [ eapply socket_handlers_coh_deliver_message ; eauto | eauto.. ].
+    - by rewrite lookup_insert.
+    - by rewrite lookup_insert.
+  Qed.
+
+  Lemma sent_received_at_evolution_drop_message
+        m M S a RT (mh : messages_history):
+    m ∈ M →
+    mh !! a = Some RT →
+    RT = sent_received_at_evolution M (M ∖ {[m]}) S S a RT.
+  Proof.
+    intros Hm Hmha. rewrite /sent_received_at_evolution.
+    match goal with |-  _ = default _ ?x => destruct x eqn:Heq end; last done.
+    destruct (get_buffer S a) eqn:Hbeq; last done.
+    simpl in Heq. rewrite difference_diag_L right_id_L in Heq.
+    assert (M ∖ {[m]} ∖ M = ∅) as Hest by set_solver. rewrite Hest in Heq.
+    rewrite /messages_sent_from filter_empty_L right_id_L in Heq.
+    rewrite -Heq. simpl. by destruct RT.
+  Qed.
+
+  Lemma sent_received_at_evolution_deliver_message ip Sn sh a skt r m S M RT :
+    m ∈ messages_to_receive_at a M →
+    socket_handlers_coh Sn →
+    S !! ip = Some Sn →
+    Sn !! sh = Some (skt, r) →
+    ip = ip_of_address a →
+    saddress skt = Some a →
+    RT = sent_received_at_evolution
+           M M S (<[ip:=<[sh:=(skt, r ∪ {[m]})]> Sn]> S) a RT.
+  Proof.
+    intros ??????.
+    rewrite /sent_received_at_evolution.
+    match goal with |-  _ = default _ ?x => destruct x eqn:Heq end; last done.
+    destruct (get_buffer S a) eqn:Hbeq; last done.
+    simpl in Heq. rewrite difference_diag_L in Heq.
+    rewrite /messages_sent_from filter_empty_L right_id_L in Heq.
+    simplify_eq. erewrite get_buffer_deliver_message in Heq; eauto.
+    simpl in *.
+    erewrite get_buffer_some in Hbeq; eauto.
+    simplify_eq.
+    assert (m0 ∖ (m0 ∪ {[m]}) = ∅) as -> by set_solver.
+    rewrite right_id_L. intuition.
+  Qed.
+
+  Lemma sent_received_at_evolution_ne
+        ip a a' sh skt (mh : messages_history) p Sn M S r:
+    (∀ ip Sn, S !! ip = Some Sn → socket_handlers_coh Sn) →
+    mh !! a' = Some p →
+    saddress skt = Some a →
+    S !! ip = Some Sn →
+    a' ≠ a →
+    p = sent_received_at_evolution M M S (<[ip:=<[sh:=(skt, r)]> Sn]> S) a' p.
+  Proof.
+    intros Hcoh???HSn?.
+    rewrite /sent_received_at_evolution.
+    match goal with |-  _ = default _ ?x => destruct x eqn:Heq end; last done.
+    destruct (get_buffer S a') eqn:Hbeq; last done.
+    simpl in Heq. rewrite difference_diag_L in Heq.
+    rewrite /messages_sent_from filter_empty_L right_id_L in Heq.
+    destruct
+      (get_buffer (<[ip:=<[sh:=(skt, r)]> Sn]> S) a') eqn:Heq2; last done.
+    simpl in *.
+    apply get_buffer_inv in Hbeq as (sh0 & skt0 & Sn0 & HS0 & HSn0 & Hskt0).
+    apply get_buffer_inv in Heq2 as (sh1 & skt1 & Sn1 & HS1 & HSn1 & Hskt1).
+    simplify_eq /=.
+    ddeq ip (ip_of_address a').
+    - ddeq sh sh1.
+      + assert (sh0 = sh1) as ->.
+        { eapply (Hcoh (ip_of_address a') Sn HSn sh0 sh1 skt0 skt1); eauto.
+            by rewrite Hskt0 Hskt1. }
+        simplify_map_eq /=. rewrite difference_diag_L right_id_L.
+        by destruct p.
+    - assert (sh0 = sh1) as ->.
+      { eapply (Hcoh (ip_of_address a') Sn0 HS0 sh0 sh1 skt0 skt1); eauto.
+          by rewrite Hskt0 Hskt1. }
+      simplify_map_eq /=. rewrite difference_diag_L right_id_L.
+      by destruct p.
+  Qed.
+
+  Lemma message_history_evolution_deliver_message ip Sn sh a skt r m S M mh :
+    m ∈ messages_to_receive_at a M →
+    S !! ip = Some Sn →
+    Sn !! sh = Some (skt, r) →
+    ip = ip_of_address a →
+    saddress skt = Some a →
+    (∀ ip Sn, S !! ip = Some Sn → socket_handlers_coh Sn) →
+    mh =
+    message_history_evolution M M S (<[ip:=<[sh:=(skt, r ∪ {[m]})]> Sn]> S) mh.
+  Proof.
+  intros ??????Hcoh.
+  rewrite-{1}(map_imap_Some mh).
+  rewrite /message_history_evolution.
+  apply map_imap_ext.
+  intros a'.
+  destruct (mh !! a') eqn:Hmh; rewrite Hmh; last done; simpl.
+  do 2 f_equal.
+  destruct (decide (a' = a)) as [->|Hneq].
+  - specialize (Hcoh ip Sn).
+    eapply sent_received_at_evolution_deliver_message; eauto.
+  - rewrite /sent_received_at_evolution.
+      by eapply sent_received_at_evolution_ne.
+  Qed.
+
+Lemma message_history_evolution_drop_message m S M mh :
+  m ∈ M →
+  messages_history_coh M S mh →
+  mh = message_history_evolution M (M ∖ {[m]}) S S mh.
+Proof.
+  intros ??. rewrite-{1}(map_imap_Some mh).
+  rewrite /message_history_evolution. apply map_imap_ext.
+  intros a'. destruct (mh !! a') eqn:Hmh; rewrite Hmh; last done; simpl.
+  do 2 f_equal. by eapply sent_received_at_evolution_drop_message.
+Qed.
+
+End Aneris_AS.
